src/Util/FisherYates/Correctness.dfy
@@ -6,5 +6,74 @@
 module FisherYates.Correctness {
   import Permutations
   import Model
+  import Rand
+  import Uniform
+  import Monad
+  import Independence
+  import RealArith
+
+  lemma {:rlimit 1000} {:vcs_split_on_every_assert} CorrectnessFisherYates<T(!new)>(xs: seq<T>, p: seq<T>)
+    requires Permutations.IsPermutationOf(p, xs)
+    ensures
+      var e := iset s | Model.Shuffle(xs)(s).Equals(p);
+      && e in Rand.eventSpace
+      && |Permutations.CalculateAllPermutationsOf(xs)| > 0
+      && Rand.prob(e) == 1.0 / (|Permutations.CalculateAllPermutationsOf(xs)| as real)
+  {
+    var e := iset s | Model.Shuffle(xs)(s).Equals(p);
+    assume {:axiom} e in Rand.eventSpace; // todo later
+
+    if |xs| != 0 {
+      var h := Uniform.Model.IntervalSample(0, |xs|); 
+      var f :=        
+        (j: int) requires 0 <= j < |xs| => 
+          var zs := Permutations.Swap(xs, 0, j);
+          Monad.Map(Model.Shuffle(zs[1..]), (ys: seq<T>) => [zs[0]] + ys);
+
+      assert Independence.IsIndep(h) by {
+        Uniform.Correctness.IntervalSampleIsIndep(0, |xs|);
+      }    
+      var j: int := Permutations.FirstOccurrence(xs, p[0]);
+      var A: iset<int> := iset{j};
+      var A2: iset<seq<T>> := iset xs | xs[1..] == p[1..];
+      var E: iset<Rand.Bitstream> := Monad.BitstreamsWithValueIn(f(j), A2);
+      var zs := Permutations.Swap(xs, 0, j)[1..];
+      assert A1: Rand.prob(iset s | s in Monad.BitstreamsWithValueIn(h, A)) == 1.0 / |xs| as real by {
+        calc {
+          Rand.prob(iset s | s in Monad.BitstreamsWithValueIn(h, A));
+          Rand.prob(iset s | Uniform.Model.IntervalSample(0, |xs|)(s).Equals(j));
+          { Uniform.Correctness.UniformFullIntervalCorrectness(0, |xs|, j); }
+          1.0 / |xs| as real;
+        }
+      }
+      assert A2: Rand.prob(E) == 1.0 / (|Permutations.CalculateAllPermutationsOf(zs)| as real) by {
+        calc {
+          Rand.prob(E);
+          Rand.prob(Monad.BitstreamsWithValueIn(f(j), A2));
+          Rand.prob(iset s | f(j)(s).Result? && f(j)(s).value[1..] == p[1..]);
+          Rand.prob(iset s | Model.Shuffle(zs)(s).Equals(p[1..]));
+          1.0 / (|Permutations.CalculateAllPermutationsOf(zs)| as real);
+        }
+      }
+      calc {
+        Rand.prob(e);
+        Rand.prob(iset s | Model.Shuffle(xs)(s).Equals(p));
+        Rand.prob(iset s | Monad.Bind(h, f)(s).Equals(p));
+        Rand.prob(iset s | s in Monad.BitstreamsWithValueIn(h, A) && s in Monad.BitstreamsWithRestIn(h, E));
+        { Independence.ResultsIndependent(h, A, E); }
+        Rand.prob(iset s | s in Monad.BitstreamsWithValueIn(h, A)) * Rand.prob(E);
+        { reveal A1; reveal A2; }
+        (1.0 / |xs| as real) * (1.0 / |Permutations.CalculateAllPermutationsOf(zs)| as real);
+        { RealArith.SimplifyFractionsMultiplication(1.0, |xs| as real, 1.0, |Permutations.CalculateAllPermutationsOf(zs)| as real); }
+        (1.0 * 1.0) / (|xs| as real * |Permutations.CalculateAllPermutationsOf(zs)| as real);
+        { assert 1.0 * 1.0 == 1.0; assert |xs| as real * |Permutations.CalculateAllPermutationsOf(zs)| as real == (|xs| * |Permutations.CalculateAllPermutationsOf(zs)|) as real; }
+        1.0 / ((|xs| * |Permutations.CalculateAllPermutationsOf(zs)|) as real);
+        { assume {:axiom} |xs| * |Permutations.CalculateAllPermutationsOf(zs)| == |Permutations.CalculateAllPermutationsOf(xs)|; } // todo later
+        1.0 / |Permutations.CalculateAllPermutationsOf(xs)| as real;
+      }
+    } else { 
+      assume {:axiom} false; // todo later
+    }
+  }
 
 }
